src/Init/Data/Range/Polymorphic/RangeIterator.lean
@@ -432,6 +432,23 @@ theorem Iterator.isPlausibleIndirectOutput_iff
 section IteratorLoop
 
 /--
+An efficient {name}`IteratorLoopNew` instance:
+As long as the compiler cannot optimize away the {name}`Option` in the internal state, we use a special
+loop implementation.
+-/
+@[always_inline, inline]
+instance Iterator.instIteratorLoopNew [UpwardEnumerable α] [LE α] [DecidableLE α]
+    [LawfulUpwardEnumerable α] [LawfulUpwardEnumerableLE α] :
+    IteratorLoopNew (Rxc.Iterator α) Id n where
+  forInNew := IteratorLoopNew.defaultImplementation.forInNew -- TODO
+
+instance Iterator.instLawfulIteratorLoopNew [UpwardEnumerable α] [LE α] [DecidableLE α]
+    [LawfulUpwardEnumerable α] [LawfulUpwardEnumerableLE α]
+    {n : Type u → Type w} :
+    LawfulIteratorLoopNew (Rxc.Iterator α) Id n where
+  lawfulNew _ := rfl
+
+/--
 An efficient {name}`IteratorLoop` instance:
 As long as the compiler cannot optimize away the {name}`Option` in the internal state, we use a special
 loop implementation.
@@ -605,7 +622,6 @@ instance Iterator.instLawfulIteratorLoop [UpwardEnumerable α] [LE α] [Decidabl
         apply IterM.DefaultConsumers.forIn'_eq_forIn' Pl wf <;> all_goals (intros; rfl)
       · simp
     · simp
-  lawfulNew := fun _ => rfl
 
 end IteratorLoop
 
@@ -1009,6 +1025,23 @@ theorem Iterator.isPlausibleIndirectOutput_iff
 section IteratorLoop
 
 /--
+An efficient {name}`IteratorLoopNew` instance:
+As long as the compiler cannot optimize away the {name}`Option` in the internal state, we use a special
+loop implementation.
+-/
+instance Iterator.instIteratorLoopNew [UpwardEnumerable α] [LT α] [DecidableLT α]
+    [LawfulUpwardEnumerable α] [LawfulUpwardEnumerableLT α]
+    {n : Type u → Type w} :
+    IteratorLoopNew (Rxo.Iterator α) Id n where
+  forInNew := IteratorLoopNew.defaultImplementation.forInNew -- TODO
+
+instance Iterator.instLawfulIteratorLoopNew [UpwardEnumerable α] [LT α] [DecidableLT α]
+    [LawfulUpwardEnumerable α] [LawfulUpwardEnumerableLT α]
+    {n : Type u → Type w} :
+    LawfulIteratorLoopNew (Rxo.Iterator α) Id n where
+  lawfulNew _ := rfl
+
+/--
 An efficient {name}`IteratorLoop` instance:
 As long as the compiler cannot optimize away the {name}`Option` in the internal state, we use a special
 loop implementation.
@@ -1178,7 +1211,6 @@ instance Iterator.instLawfulIteratorLoop [UpwardEnumerable α] [LT α] [Decidabl
         apply IterM.DefaultConsumers.forIn'_eq_forIn' Pl wf <;> all_goals (intros; rfl)
       · simp
     · simp
-  lawfulNew := fun _ => rfl
 
 end IteratorLoop
 
@@ -1496,6 +1528,23 @@ theorem Iterator.isPlausibleIndirectOutput_iff
 section IteratorLoop
 
 /--
+An efficient {name}`IteratorLoopNew` instance:
+As long as the compiler cannot optimize away the {name}`Option` in the internal state, we use a special
+loop implementation.
+-/
+instance Iterator.instIteratorLoopNew [UpwardEnumerable α]
+    [LawfulUpwardEnumerable α]
+    {n : Type u → Type w} :
+    IteratorLoopNew (Rxi.Iterator α) Id n where
+  forInNew := IteratorLoopNew.defaultImplementation.forInNew -- TODO
+
+instance Iterator.instLawfulIteratorLoopNew [UpwardEnumerable α]
+    [LawfulUpwardEnumerable α]
+    {n : Type u → Type w} :
+    LawfulIteratorLoopNew (Rxi.Iterator α) Id n where
+  lawfulNew _ := rfl
+
+/--
 An efficient {name}`IteratorLoop` instance:
 As long as the compiler cannot optimize away the {name}`Option` in the internal state, we use a special
 loop implementation.
@@ -1643,7 +1692,6 @@ instance Iterator.instLawfulIteratorLoop [UpwardEnumerable α]
       rw [← IterM.DefaultConsumers.forIn'_eq_wf Pl wf _]
       apply IterM.DefaultConsumers.forIn'_eq_forIn' Pl wf <;> all_goals (intros; rfl)
     · simp
-  lawfulNew := fun _ => rfl
 
 end IteratorLoop
 
